common/AST.v
@@ -465,10 +465,12 @@ Inductive external_function : Type :=
          used with caution, as it can invalidate the semantic
          preservation theorem.  Generated only if [-finline-asm] is
          given. *)
-  | EF_debug (kind: positive) (text: ident) (targs: list typ).
+  | EF_debug (kind: positive) (text: ident) (targs: list typ)
      (** Transport debugging information from the front-end to the generated
          assembly.  Takes zero, one or several arguments like [EF_annot].
          Unlike [EF_annot], produces no observable event. *)
+  | EF_realize.
+     (** Realize a memory chunk. *)
 
 (** The type signature of an external function. *)
 
@@ -486,6 +488,7 @@ Definition ef_sig (ef: external_function): signature :=
   | EF_annot_val text targ => mksignature (targ :: nil) (Some targ) cc_default
   | EF_inline_asm text sg clob => sg
   | EF_debug kind text targs => mksignature targs None cc_default
+  | EF_realize => mksignature (Tptr :: nil) None cc_default
   end.
 
 (** Whether an external function should be inlined by the compiler. *)
@@ -504,6 +507,7 @@ Definition ef_inline (ef: external_function) : bool :=
   | EF_annot_val text targ => true
   | EF_inline_asm text sg clob => true
   | EF_debug kind text targs => true
+  | EF_realize => true
   end.
 
 (** Whether an external function must reload its arguments. *)
